Checkpoint more indirect block sm progress
Finish with indclear

src/BlockPtr.v
@@ -201,7 +201,7 @@ Module BlockPtr (BPtr : BlockPtrSig).
     | 0 => indrep_n_helper Fs bxp ibn l
     | S indlvl' =>
       exists iblocks Fs' lFs,
-        [[ length lFs = NIndirect ]] *
+        [[ length lFs = length iblocks ]] *
         [[ Fs <=p=> Fs' * pred_fold_left lFs ]] *
         indrep_n_helper Fs' bxp ibn iblocks *
         exists l_part, [[ l = concat l_part ]] *
@@ -213,6 +213,7 @@ Module BlockPtr (BPtr : BlockPtrSig).
   Hint Extern 0 (okToUnify (indrep_n_tree _ _ _ _ _) (indrep_n_tree _ _ _ _ _ )) => constructor : okToUnify.
   Local Hint Extern 0 (okToUnify (listmatch _ ?a _) (listmatch _ ?a _)) => constructor : okToUnify.
   Local Hint Extern 0 (okToUnify (listmatch _ _ ?b) (listmatch _ _ ?b)) => constructor : okToUnify.
+  Local Hint Extern 0 (okToUnify (listmatch _ (combine ?a _) _) (listmatch _ (combine ?a _) _)) => constructor : okToUnify.
 
   (* Necessary to make subst work when there's a recursive term like:
      l = firstn (length l) ... *)
@@ -321,6 +322,12 @@ Module BlockPtr (BPtr : BlockPtrSig).
     unfold indrep_n_helper; intros; split; cancel.
   Qed.
 
+  Lemma indrep_n_helper_0' : forall bxp l,
+    indrep_n_helper emp bxp 0 l <=p=> [[ l = repeat $0 NIndirect ]].
+  Proof.
+    unfold indrep_n_helper; intros; split; cancel.
+  Qed.
+
   Lemma pred_fold_left_Forall_emp: forall AT AEQ V (l : list (@pred AT AEQ V)),
     Forall (fun x => x <=p=> emp) l ->
     pred_fold_left l <=p=> emp.
@@ -360,6 +367,44 @@ Module BlockPtr (BPtr : BlockPtrSig).
     intros.
     rewrite pred_fold_left_Forall_emp; auto.
     auto using Forall_repeat.
+  Qed.
+
+  Lemma pred_fold_left_app: forall AT AEQ V (l l' : list (@pred AT AEQ V)),
+    pred_fold_left (l ++ l') <=p=> pred_fold_left l * pred_fold_left l'.
+  Proof.
+    induction l; intros.
+    split; cancel.
+    intros.
+    cbn [app].
+    repeat rewrite pred_fold_left_cons.
+    rewrite IHl.
+    split; cancel.
+  Qed.
+
+  Lemma pred_fold_left_selN_removeN: forall AT AEQ V (l : list (@pred AT AEQ V)) i,
+    pred_fold_left l <=p=> (selN l i emp) * pred_fold_left (removeN l i).
+  Proof.
+    unfold removeN.
+    intros.
+    destruct (lt_dec i (length l)).
+    rewrite <- firstn_skipn with (l := l) at 1.
+    repeat rewrite pred_fold_left_app.
+    erewrite skipn_selN_skipn by eauto.
+    rewrite pred_fold_left_cons.
+    split; cancel.
+    rewrite selN_oob, firstn_oob, skipn_oob by omega.
+    rewrite app_nil_r.
+    split; cancel.
+  Qed.
+
+  Lemma pred_fold_left_updN_removeN: forall AT AEQ V l (p : @pred AT AEQ V) i,
+    i < length l ->
+    pred_fold_left (updN l i p) <=p=> pred_fold_left (removeN l i) * p.
+  Proof.
+    intros.
+    rewrite pred_fold_left_selN_removeN.
+    rewrite selN_updN_eq, removeN_updN by auto.
+    split; cancel.
   Qed.
 
   Theorem indrep_n_tree_0 : forall indlvl bxp Fs l,
@@ -429,15 +474,13 @@ Module BlockPtr (BPtr : BlockPtrSig).
     apply Forall_repeat. auto.
   Qed.
 
-  Lemma listmatch_indrep_n_tree_empty: forall indlvl bxp,
-    let iblocks := (repeat $0 NIndirect) in
-    indrep_n_helper emp bxp 0 iblocks *
+  Lemma listmatch_indrep_n_tree_empty': forall indlvl n bxp,
     listmatch (fun x y => indrep_n_tree indlvl bxp (snd x) # (fst x) y)
-      (combine iblocks (repeat emp NIndirect)) (repeat (repeat $0 (NIndirect ^ (S indlvl))) NIndirect) <=p=> emp.
+      (combine (repeat (@natToWord addrlen 0) n) (repeat emp n)) (repeat (repeat $0 (NIndirect ^ (S indlvl))) n) <=p=> emp.
   Proof.
-    cbn -[Nat.div]; intros.
+    intros.
     rewrite listmatch_emp_piff.
-    rewrite combine_length_eq; autorewrite with lists; eauto.
+    autorewrite with lists; auto.
     split; cancel.
     intros.
     rewrite combine_repeat in *.
@@ -445,6 +488,61 @@ Module BlockPtr (BPtr : BlockPtrSig).
     eapply repeat_spec in H0.
     subst.
     rewrite indrep_n_tree_0.
+    split; cancel.
+  Qed.
+
+  Lemma in_combine_repeat_l : forall A B (a : A) n (b : list B) x,
+    In x (combine (repeat a n) b) ->
+    fst x = a.
+  Proof.
+    induction n; cbn; intuition.
+    destruct b; cbn in *; intuition eauto.
+    subst; auto.
+  Qed.
+
+  Lemma listmatch_indrep_n_tree_empty'': forall indlvl n fsl l bxp,
+    length fsl = n ->
+    listmatch (fun x y => indrep_n_tree indlvl bxp (snd x) # (fst x) y)
+      (combine (repeat (@natToWord addrlen 0) n) fsl) l =p=> [[ pred_fold_left fsl <=p=> emp ]] *
+        [[ l = (repeat (repeat $0 (NIndirect ^ (S indlvl))) n) ]].
+  Proof.
+    cbn -[Nat.div]; intros.
+    rewrite listmatch_lift_l with (P := fun x => snd x <=p=> emp).
+    erewrite listmatch_lift_r with (P := fun x => x = repeat $0 (NIndirect ^ (S indlvl))).
+    rewrite listmatch_emp_piff.
+    autorewrite with lists.
+    rewrite Nat.min_l by omega.
+    do 2 intro; destruct_lifts.
+    - repeat eapply sep_star_lift_apply'; unfold lift_empty; intuition.
+      rewrite Forall_combine_r in H1.
+      rewrite pred_fold_left_Forall_emp; eauto.
+      autorewrite with lists; eauto.
+      reflexivity.
+      eapply list_selN_ext.
+      autorewrite with lists; auto.
+      intros.
+      rewrite Forall_forall in *.
+      rewrite H2 with (x := selN l pos nil).
+      rewrite repeat_selN; auto; omega.
+      eapply in_selN; auto.
+    - instantiate (1 := fun x y => emp).
+      auto.
+    - instantiate (1 := fun x y => ([[ y = repeat $0 (NIndirect ^ (S indlvl)) ]])%pred).
+      split; cancel.
+    - intros.
+      erewrite in_combine_repeat_l in * by eauto.
+      rewrite indrep_n_tree_0.
+      split; cancel.
+  Qed.
+
+  Lemma listmatch_indrep_n_tree_empty: forall indlvl bxp,
+    let iblocks := (repeat $0 NIndirect) in
+    indrep_n_helper emp bxp 0 iblocks *
+    listmatch (fun x y => indrep_n_tree indlvl bxp (snd x) # (fst x) y)
+      (combine iblocks (repeat emp NIndirect)) (repeat (repeat $0 (NIndirect ^ (S indlvl))) NIndirect) <=p=> emp.
+  Proof.
+    cbn -[Nat.div]; intros.
+    rewrite listmatch_indrep_n_tree_empty'.
     split; cancel.
   Qed.
 
@@ -530,9 +628,9 @@ Module BlockPtr (BPtr : BlockPtrSig).
   Qed.
 
   Local Hint Extern 1 (Forall (fun x => length x = _) _) => match goal with
-    | [H : context [listmatch (fun x y => indrep_n_tree _ (fst x) # (snd x) y) _ ?l]
+    | [H : context [listmatch (fun x y => indrep_n_tree _ _ (snd x) # (fst x) y) _ ?l]
         |- Forall (fun x => length x = _) ?l ] =>
-          rewrite listmatch_indrep_n_tree_forall_length in H; destruct_lift H; solve [eassumption]
+          rewrite listmatch_indrep_n_tree_forall_length with (l2 := l) in H; destruct_lift H; solve [eassumption]
     | [|- Forall _ (upd_range ?l _ _ _)] => apply forall_upd_range; autorewrite with lists; eauto
   end.
 
@@ -731,14 +829,6 @@ Module BlockPtr (BPtr : BlockPtrSig).
     cancel.
   Qed.
 
-  Lemma in_combine_repeat_l : forall A B (a : A) n (b : list B) x,
-    In x (combine (repeat a n) b) ->
-    fst x = a.
-  Proof.
-    induction n; cbn; intuition.
-    destruct b; cbn in *; intuition eauto.
-    subst; auto.
-  Qed.
 
   Theorem xform_indrep_n_helper : forall Fs bxp ir l,
     crash_xform (indrep_n_helper Fs bxp ir l) <=p=> indrep_n_helper Fs bxp ir l.
@@ -790,28 +880,47 @@ Module BlockPtr (BPtr : BlockPtrSig).
       replace (length l) with NIndirect in * by (rewrite indrep_n_helper_length_piff in H; destruct_lift H; auto)
     | [ |- ?off / ?N < ?N' ] => apply Nat.div_lt_upper_bound; [ mult_nonzero |]
     | [ |- ?off < ?N * NIndirect] => rewrite mult_comm
+    | [ H: context [length (combine ?a ?b)] |- _ ]=>
+      replace (length (combine a b)) with (Nat.min (length a) (length b)) in * by
+        (rewrite combine_length; reflexivity)
+    | [ |- context [length (combine ?a ?b)] ]=>
+      replace (length (combine a b)) with (Nat.min (length a) (length b)) in * by
+        (rewrite combine_length; reflexivity)
+
     (* try to get an argument to indrep_n_tree or indrep_n_helper *)
-    | [ H : context [listmatch _ (combine ?a ?b) ?c], H' : context [length ?c] |- _ ] =>
-      replace (length c) with (length a) in * by (rewrite listmatch_combine_l_length in H; destruct_lift H; omega)
-    | [ H : context [listmatch _ (combine ?a ?b) ?c], H' : context [length ?c] |- _ ] =>
-      replace (length c) with (length b) in * by (rewrite listmatch_combine_l_length in H; destruct_lift H; omega)
-    | [ H : context [listmatch _ (combine ?a ?b) ?c] |- context [length ?c] ] =>
-      replace (length c) with (length a) in * by (rewrite listmatch_combine_l_length in H; destruct_lift H; omega)
-    | [ H : context [listmatch _ (combine ?a ?b) ?c] |- context [length ?c] ] =>
-      replace (length c) with (length b) in * by (rewrite listmatch_combine_l_length in H; destruct_lift H; omega)
-    | [ H : context [listmatch _ ?a ?b] |- context [length ?b] ] =>
-      replace (length b) with (length a) in * by (rewrite listmatch_length_pimpl in H; destruct_lift H; auto)
+    | [ H : context [listmatch _ (combine ?A _) ?c], H' : context [length ?c] |- _ ] =>
+      replace (length c) with (length A) in * by (
+        rewrite listmatch_combine_l_length with (a := A) in H; destruct_lift H; omega)
+    | [ H : context [listmatch _ (combine _ ?B) ?c], H' : context [length ?c] |- _ ] =>
+      replace (length c) with (length B) in * by (
+        rewrite listmatch_combine_l_length with (b := B) in H; destruct_lift H; omega)
+
+    | [ H : context [listmatch _ (combine ?A _) ?c] |- context [length ?c] ] =>
+      replace (length c) with (length A) in * by (
+        rewrite listmatch_combine_l_length with (a := A) in H; destruct_lift H; omega)
+    | [ H : context [listmatch _ (combine _ ?B) ?c] |- context [length ?c] ] =>
+      replace (length c) with (length B) in * by (
+        rewrite listmatch_combine_l_length with (b := B) in H; destruct_lift H; omega)
+
+    | [ H : context [listmatch _ ?A ?b] |- context [length ?b] ] =>
+      replace (length b) with (length A) in * by (
+        rewrite listmatch_length_pimpl with (a := A) in H; destruct_lift H; auto)
+    | [ H : context [listmatch _ ?A ?b], H': context [length ?b] |- _ ] =>
+      replace (length b) with (length A) in * by (
+        rewrite listmatch_length_pimpl with (a := A) in H; destruct_lift H; auto)
+
     | [ H : context [lift_empty _] |- _ ] => progress destruct_lift H
     | [ H : context [length (concat ?l)] |- _ ] => erewrite concat_hom_length in H by eauto
     | [ |- context [length (concat _)] ] => rewrite concat_hom_length by eauto
     | [ |- context [Nat.min _ _] ] => rewrite min_l by omega
     | [ H: context [Nat.min _ _] |- _ ] => rewrite min_l in H by omega
     | [ |- _ ] => omega
+    | [ |- ?a < ?b * ?c ] => rewrite mult_comm; omega
     end.
 
   Ltac indrep_n_tree_bound :=
     match goal with
-    | [l : list _ |- context [?x] ] => is_evar x; unify x l; indrep_n_tree_bound
+    | [l : list _ |- context [?x] ] => is_evar x; unify x l; solve [indrep_n_tree_bound]
     | _ => repeat indrep_n_tree_bound_step
   end.
 
@@ -823,6 +932,9 @@ Module BlockPtr (BPtr : BlockPtrSig).
       end
     | [|- context [selN ?l ?n] ] => rewrite listmatch_isolate with (i := n) (a := l);
         autorewrite with lists in *; try omega; try erewrite snd_pair by eauto
+    | [|- context [selN ?l ?n] ] => rewrite listmatch_isolate with (i := n) (a := combine l _);
+        autorewrite with lists in *; try rewrite selN_combine; try omega; try erewrite snd_pair by eauto;
+        cbn [fst snd] in *
   end.
 
   Ltac indrep_n_tree_extract_lengths :=
@@ -1224,60 +1336,130 @@ Module BlockPtr (BPtr : BlockPtrSig).
 
   Local Hint Extern 1 ({{_}} Bind (indclear_all _ _ _ _ _ ) _) => apply indclear_all_ok : prog.
 
-  Definition indclear_aligned indlvl lxp bxp indbns start len ms :=
+  Definition indclear_aligned indlvl lxp bxp (indbns : list waddr) start len ms :=
     let N := NIndirect ^ S indlvl in
-    ForN i < len / N
+    let indbns := firstn (len / N) (skipn (start / N) indbns) in
+    ForEach bn rest indbns
       Hashmap hm
-      Ghost [ F Fm l_part bxp crash m0 freelist ]
+      Ghost [ F Fm Fs l_part fsl bxp crash m0 sm freelist ]
       Loopvar [ ms ]
       Invariant
-        exists l_part' indbns' freelist' m,
-        LOG.rep lxp F (LOG.ActiveTxn m0 m) (BALLOCC.MSLog ms) hm *
-        [[ l_part' = upd_range l_part (start / N) i (repeat $0 N) ]] *
-        [[ indbns' = upd_range indbns (start / N) i $0 ]] *
-        [[[ m ::: Fm * listmatch (fun ibn' l' => indrep_n_tree indlvl bxp (# ibn') l') indbns' l_part' *
+        exists l_part' indbns' fsl' freelist' m,
+        LOG.rep lxp F (LOG.ActiveTxn m0 m) (BALLOCC.MSLog ms) sm hm *
+        let n := length indbns - length rest in
+        [[ l_part' = skipn n l_part ]] *
+        [[ indbns' = skipn n indbns ]] *
+        [[ fsl' = skipn n fsl ]] *
+        [[[ m ::: Fm * listmatch (fun x l' => indrep_n_tree indlvl bxp (snd x) # (fst x) l') (combine indbns' fsl') l_part' *
                   BALLOCC.rep bxp freelist' ms ]]] *
+        [[ (Fs * pred_fold_left fsl' * BALLOCC.smrep freelist')%pred sm ]] *
         [[ incl freelist freelist' ]]
       OnCrash crash
       Begin
-        ms <- indclear_all indlvl lxp bxp #(selN indbns (i + start / N) IndRec.Defs.item0) ms;
+        ms <- indclear_all indlvl lxp bxp # bn ms;
         Ret ^(ms)
       Rof ^(ms).
 
   Theorem indclear_aligned_ok : forall indlvl lxp bxp indbns start len ms,
     let N := NIndirect ^ S indlvl in
-    {< F Fm m0 m l_part freelist,
+    {< F Fm Fs m0 sm m l_part fsl freelist,
     PRE:hm
-           LOG.rep lxp F (LOG.ActiveTxn m0 m) (BALLOCC.MSLog ms) hm *
-           [[[ m ::: (Fm * listmatch (fun ibn l => indrep_n_tree indlvl bxp (#ibn) l) indbns l_part
+           LOG.rep lxp F (LOG.ActiveTxn m0 m) (BALLOCC.MSLog ms) sm hm *
+           [[[ m ::: (Fm * listmatch (fun x l => indrep_n_tree indlvl bxp (snd x) # (fst x) l) (combine indbns fsl) l_part
                          * BALLOCC.rep bxp freelist ms) ]]] *
-           [[ start / N + len / N <= length l_part ]] * [[ Nat.divide N start ]] * [[ Nat.divide N len ]]
+           [[ start / N + len / N <= length l_part ]] * [[ Nat.divide N start ]] * [[ Nat.divide N len ]] *
+           [[ length fsl = length indbns ]] *
+           [[ (Fs * BALLOCC.smrep freelist * pred_fold_left fsl)%pred sm ]]
     POST:hm' RET:^(ms)
-           exists m' freelist' indbns' l_part', 
-           LOG.rep lxp F (LOG.ActiveTxn m0 m') (BALLOCC.MSLog ms) hm' *
-           [[[ m' ::: (Fm * listmatch (fun ibn l => indrep_n_tree indlvl bxp (#ibn) l) indbns' l_part'
+           exists m' freelist' indbns' fsl' l_part', 
+           LOG.rep lxp F (LOG.ActiveTxn m0 m') (BALLOCC.MSLog ms) sm hm' *
+           [[[ m' ::: (Fm * listmatch (fun x l => indrep_n_tree indlvl bxp (snd x) #(fst x) l) (combine indbns' fsl') l_part'
                           * BALLOCC.rep bxp freelist' ms) ]]] *
            [[ indbns' = upd_range indbns (start / N) (len / N) $0 ]] *
            [[ l_part' = upd_range l_part (start / N) (len / N) (repeat $0 N) ]] *
-           [[ incl freelist freelist' ]]
-    CRASH:hm'  LOG.intact lxp F m0 hm'
+           [[ incl freelist freelist' ]] *
+           [[ length fsl' = length indbns' ]] *
+           [[ (Fs * BALLOCC.smrep freelist' * pred_fold_left fsl')%pred sm ]]
+    CRASH:hm'  LOG.intact lxp F m0 sm hm'
     >} indclear_aligned indlvl lxp bxp indbns start len ms.
     Proof.
       unfold indclear_aligned. unfold Nat.divide.
       prestep. norml.
       repeat rewrite Nat.div_mul in * by mult_nonzero.
       rewrite listmatch_length_pimpl in *. destruct_lifts.
-      cancel; hoare.
-      - rewrite listmatch_extract.
-        repeat rewrite upd_range_selN_oob. cancel.
-        all : autorewrite with lists; omega.
-      - rewrite listmatch_updN_removeN. rewrite roundTrip_0.
-        repeat rewrite indrep_n_tree_0. cancel.
-        repeat rewrite removeN_upd_range_l.
-        rewrite plus_comm. repeat rewrite removeN_upd_range_r.
-        erewrite <- removeN_upd_range_mid with (l := indbns).
-        erewrite <- removeN_upd_range_mid with (l := l_part). cancel.
-        all : autorewrite with lists; omega.
+      cancel.
+      all: repeat rewrite Nat.sub_diag; auto.
+      - cbn [skipn].
+        rewrite <- firstn_combine_comm.
+        rewrite <- skipn_combine by eauto.
+        rewrite listmatch_split with (n := z0).
+        rewrite listmatch_split with (n := z) (a := skipn _ _).
+        repeat cancel.
+      - cbn [skipn].
+        erewrite <- firstn_skipn with (n := z0) (l := fsl) at 1.
+        erewrite <- firstn_skipn with (n := z) (l := skipn _ fsl) at 1.
+        repeat rewrite pred_fold_left_app. cancel.
+      - safestep.
+        all: assert (length (firstn z (skipn z0 fsl)) = length (firstn z (skipn z0 indbns))) by
+          (repeat rewrite ?firstn_length, ?skipn_length; congruence).
+        all: assert (length (firstn z (skipn z0 l_part)) = length (firstn z (skipn z0 indbns))) by
+          (rewrite firstn_length, skipn_length; indrep_n_tree_bound).
+        all: assert (length prefix < length (firstn z (skipn z0 indbns))) by
+          (substl (firstn z (skipn z0 indbns)); rewrite app_length; cbn; omega).
+        repeat rewrite <- H5 in *.
+        autorewrite with lists; cbn [length].
+        repeat rewrite Nat.add_sub.
+        rewrite skipn_app.
+        + erewrite skipn_selN_skipn with (l := firstn _ (skipn _ fsl)) at 1.
+          erewrite skipn_selN_skipn with (l := firstn _ (skipn _ l_part)) at 1.
+          cbn [combine].
+          rewrite listmatch_cons.
+          cancel.
+          all: omega.
+        + repeat rewrite <- H5 in *.
+          autorewrite with lists; cbn [length].
+          rewrite Nat.add_sub.
+          erewrite skipn_selN_skipn with (off := length prefix).
+          rewrite pred_fold_left_cons.
+          cancel. reflexivity.
+          omega.
+        + step.
+          repeat rewrite <- H5.
+          autorewrite with lists. cbn [length].
+          repeat match goal with |- context [?b + S ?a - ?a] => replace (b + S a - a) with (b + 1) by omega end.
+          rewrite skipn_app_r_ge by omega.
+          rewrite minus_plus. rewrite <- plus_n_Sm, <- plus_n_O.
+          rewrite indrep_n_tree_0.
+          cancel.
+          repeat rewrite <- H5.
+          autorewrite with lists. cbn [length].
+          repeat match goal with |- context [?b + S ?a - ?a] => replace (b + S a - a) with (b + 1) by omega end.
+          rewrite <- plus_n_Sm, <- plus_n_O.
+          cancel.
+        + cancel.
+      - step.
+        repeat rewrite upd_range_eq_upd_range' by indrep_n_tree_bound.
+        unfold upd_range'.
+        repeat rewrite combine_app.
+        repeat rewrite skipn_skipn.
+        replace (z0 + z) with (z + z0) in * by omega.
+        rewrite firstn_combine_comm, skipn_combine by auto.
+        repeat rewrite <- listmatch_app; cancel.
+        repeat rewrite Nat.sub_0_r.
+        repeat rewrite skipn_oob by indrep_n_tree_bound.
+        rewrite listmatch_indrep_n_tree_empty'.
+        unfold listmatch; cancel.
+        autorewrite with lists; auto.
+        indrep_n_tree_bound.
+        autorewrite with lists.
+        rewrite firstn_length_l, skipn_length by indrep_n_tree_bound.
+        indrep_n_tree_bound.
+        repeat rewrite pred_fold_left_app.
+        cancel.
+        rewrite skipn_skipn.
+        rewrite skipn_oob by indrep_n_tree_bound.
+        rewrite pred_fold_left_repeat_emp.
+        cancel.
       - cancel.
         eauto using LOG.intact_hashmap_subset.
     Grab Existential Variables. all : eauto; split.
@@ -1297,30 +1479,64 @@ Module BlockPtr (BPtr : BlockPtrSig).
         Ret ^(BALLOCC.upd_memstate lms ms, bn)
       }
     }.
+Lemma indrep_n_helper_valid_sm: forall Fs bxp ir l,
+  ir <> 0 ->
+  indrep_n_helper Fs bxp ir l =p=> indrep_n_helper Fs bxp ir l * [[ Fs <=p=> ir |->? ]].
+Proof.
+  unfold indrep_n_helper.
+  intros.
+  destruct addr_eq_dec; try congruence.
+  cancel.
+Qed.
 
   Theorem update_block_ok : forall lxp bxp ir indbns indbns' ms,
-    {< F Fm m0 m freelist,
+    {< F Fm Fs IFs m0 sm m freelist,
     PRE:hm
-           LOG.rep lxp F (LOG.ActiveTxn m0 m) (BALLOCC.MSLog ms) hm *
+           LOG.rep lxp F (LOG.ActiveTxn m0 m) (BALLOCC.MSLog ms) sm hm *
             [[ BALLOCC.bn_valid bxp ir ]] *
             [[ IndRec.items_valid ir indbns' ]] *
-           [[[ m ::: (Fm * indrep_n_helper Fs bxp ir indbns) *
-              BALLOCC.rep bxp freelist ms ]]]
+           [[[ m ::: (Fm * indrep_n_helper IFs bxp ir indbns) *
+              BALLOCC.rep bxp freelist ms ]]] *
+            [[ (Fs * BALLOCC.smrep freelist * IFs)%pred sm ]]
     POST:hm' RET: ^(ms, ir')
-           exists m' freelist', 
-           LOG.rep lxp F (LOG.ActiveTxn m0 m') (BALLOCC.MSLog ms) hm' *
-           [[[ m' ::: (Fm * indrep_n_helper Fs bxp ir' indbns' *
+           exists m' freelist' IFs',
+           LOG.rep lxp F (LOG.ActiveTxn m0 m') (BALLOCC.MSLog ms) sm hm' *
+           [[[ m' ::: (Fm * indrep_n_helper IFs' bxp ir' indbns' *
               BALLOCC.rep bxp freelist' ms) ]]] *
+           [[ (Fs * BALLOCC.smrep freelist' * IFs')%pred sm ]] *
            [[ incl freelist freelist' ]] *
            ([[ ir' = 0 ]] \/ [[ ir' = ir ]])
-    CRASH:hm'  LOG.intact lxp F m0 hm'
+    CRASH:hm'  LOG.intact lxp F m0 sm hm'
     >} update_block lxp bxp ir indbns indbns' ms.
   Proof.
     unfold update_block.
-    hoare; unfold BALLOCC.bn_valid in *; intuition.
-    - rewrite indrep_n_helper_pts_piff by auto. rewrite indrep_n_helper_0. cancel.
-    - rewrite indrep_n_helper_valid by auto. cancel.
-    - rewrite indrep_n_helper_valid by auto. cancel.
+    prestep. norml.
+    assert (ir <> 0) by (unfold BALLOCC.bn_valid in *; intuition).
+    rewrite indrep_n_helper_valid_sm in * by auto.
+    denote lift_empty as Hf; destruct_lift Hf.
+    denote IFs as Hf; rewrite Hf in *.
+    denote BALLOCC.smrep as Hs; destruct_lift Hs.
+    step.
+    rewrite indrep_n_helper_pts_piff by auto. cancel.
+    + step.
+      rewrite indrep_n_helper_0 by auto.
+      cancel.
+    + prestep. norm. repeat cancel.
+      intuition idtac.
+      pred_apply. cancel.
+      pred_apply; cancel.
+      rewrite Hf; cancel.
+      auto.
+      eauto.
+    + step.
+      rewrite indrep_n_helper_valid by auto; cancel.
+      prestep. norm. repeat cancel.
+      intuition idtac.
+      rewrite indrep_n_helper_valid by auto.
+      pred_apply; cancel; eauto.
+      rewrite Hf; pred_apply; cancel.
+      auto.
+      eauto.
   Qed.
 
   Local Hint Extern 1 ({{_}} Bind (update_block _ _ _ _ _ _) _) => apply update_block_ok : prog.
@@ -1352,37 +1568,51 @@ Module BlockPtr (BPtr : BlockPtrSig).
         end
       }
     }.
-
+Lemma concat_repeat: forall T n k (x : T),
+  concat (repeat (repeat x k) n) = repeat x (n * k).
+Proof.
+  intros.
+  erewrite concat_hom_repeat.
+  autorewrite with lists.
+  eauto.
+  apply Forall_repeat; auto.
+Qed.
   Theorem indclear_from_aligned_ok : forall indlvl lxp bxp indbns start len ms,
     let N := NIndirect ^ S indlvl in
-    {< F Fm m0 m l_part freelist,
+    {< F Fm Fs m0 sm m l_part freelist fsl,
     PRE:hm
-           LOG.rep lxp F (LOG.ActiveTxn m0 m) (BALLOCC.MSLog ms) hm *
-           [[[ m ::: (Fm * listmatch (fun ibn l => indrep_n_tree indlvl bxp (#ibn) l) indbns l_part
+           LOG.rep lxp F (LOG.ActiveTxn m0 m) (BALLOCC.MSLog ms) sm hm *
+           [[[ m ::: (Fm * listmatch (fun x l => indrep_n_tree indlvl bxp (snd x) #(fst x) l) (combine indbns fsl) l_part
                          * BALLOCC.rep bxp freelist ms) ]]] *
-           [[ start + len <= length (concat l_part) ]] * [[ Nat.divide N start ]] * [[ len < N ]]
+           [[ start + len <= length (concat l_part) ]] * [[ Nat.divide N start ]] * [[ len < N ]] *
+           [[ length fsl = length indbns ]] *
+           [[ (Fs * pred_fold_left fsl * BALLOCC.smrep freelist)%pred sm ]]
     POST:hm' RET:^(ms, indbns')
-           exists m' freelist' l_part', 
-           LOG.rep lxp F (LOG.ActiveTxn m0 m') (BALLOCC.MSLog ms) hm' *
-           [[[ m' ::: (Fm * listmatch (fun ibn l => indrep_n_tree indlvl bxp (#ibn) l) indbns' l_part'
+           exists m' freelist' l_part' fsl',
+           LOG.rep lxp F (LOG.ActiveTxn m0 m') (BALLOCC.MSLog ms) sm hm' *
+           [[[ m' ::: (Fm * listmatch (fun x l => indrep_n_tree indlvl bxp (snd x) #(fst x) l) (combine indbns' fsl') l_part'
                           * BALLOCC.rep bxp freelist' ms) ]]] *
            [[ concat (l_part') = upd_range (concat l_part) start len $0 ]] *
-           [[ incl freelist freelist' ]]
-    CRASH:hm'  LOG.intact lxp F m0 hm'
+           [[ length indbns' = length indbns ]] *
+           [[ length fsl' = length indbns' ]] *
+           [[ incl freelist freelist' ]] *
+           [[ (Fs * pred_fold_left fsl' * BALLOCC.smrep freelist')%pred sm ]]
+    CRASH:hm'  LOG.intact lxp F m0 sm hm'
     >} indclear_from_aligned indlvl lxp bxp indbns start len ms.
   Proof.
     induction indlvl.
     + simpl. step; [> solve [hoare] |].
       pose proof listmatch_indrep_n_tree_forall_length 0 as H'.
-      simpl in H'. rewrite H' in *. destruct_lifts. rewrite mult_1_r in *.
+      simpl in H'. rewrite H' in *.
+      denote combine as Hc. destruct_lift Hc. rewrite mult_1_r in *.
       prestep. norml.
-      assert (start / NIndirect < length l_part).
-        indrep_n_tree_bound. rewrite mult_comm. omega.
-      assert (start / NIndirect < length indbns).
-        indrep_n_tree_bound. rewrite mult_comm. omega.
+      assert (start / NIndirect < length l_part) by indrep_n_tree_bound.
+      assert (start / NIndirect < length indbns) by indrep_n_tree_bound.
       cancel.
       - hoare.
         rewrite listmatch_extract in *.
+        erewrite selN_combine in * by auto.
+        cbn [fst snd] in *.
         denote (# _ = _) as Ha. rewrite Ha in *.
         rewrite indrep_n_helper_0 in *.
         destruct_lifts.
@@ -1390,68 +1620,105 @@ Module BlockPtr (BPtr : BlockPtrSig).
         denote (selN _ _ _ = repeat _ _) as Hb. rewrite Hb.
         rewrite upd_range_same by omega.
         erewrite selN_eq_updN_eq; eauto.
-        auto.
+        indrep_n_tree_bound.
       - step.
-        indrep_n_extract; try omega. rewrite indrep_n_helper_valid by eauto. cancel.
-        rewrite firstn_oob. hoare.
+        indrep_n_extract.
+        rewrite indrep_n_helper_valid by eauto. cancel.
+        indrep_n_tree_bound.
+        rewrite firstn_oob.
+        safestep.
+        1, 2: match goal with |- context [selN ?l ?ind ?d] =>
+            erewrite listmatch_extract with (a := combine l _) (i := ind) (ad := (d, _)) in *
+          end; rewrite ?selN_combine in * by auto; cbn [fst snd] in *;
+          auto; indrep_n_tree_bound.
+        * rewrite indrep_n_helper_items_valid in * by auto; destruct_lifts.
+          cbv [IndRec.items_valid] in *.
+          autorewrite with lists. intuition eauto.
+        * indrep_n_extract. cancel. indrep_n_tree_bound.
+        * rewrite pred_fold_left_selN_removeN with (i := start / NIndirect).
+          cancel. reflexivity.
+        * step.
+        **  rewrite combine_updN, listmatch_updN_removeN. cancel. all: indrep_n_tree_bound.
+        **  erewrite upd_range_concat_hom_start_aligned; eauto. omega.
+        **  indrep_n_tree_bound.
+        **  autorewrite with lists; omega.
+        **  rewrite pred_fold_left_selN_removeN with (l := updN _ _ _).
+            rewrite selN_updN_eq, removeN_updN by omega. cancel.
+        **  rewrite natToWord_wordToNat. rewrite combine_updN.
+            rewrite listmatch_updN_removeN by (eauto; indrep_n_tree_bound). cancel.
+        **  erewrite upd_range_concat_hom_start_aligned by (eauto; omega). auto.
+        **  indrep_n_tree_bound.
+        **  autorewrite with lists; omega.
+        **  rewrite pred_fold_left_selN_removeN with (l := updN _ _ _).
+            rewrite selN_updN_eq, removeN_updN by omega. cancel.
+        * cancel.
         * match goal with |- context [selN ?l ?ind ?d] =>
-            rewrite listmatch_extract with (a := l) (i := ind) (ad := d) in * by omega
-          end. auto.
-        * match goal with |- context [selN ?l ?ind ?d] =>
-            rewrite listmatch_extract with (a := l) (i := ind) (ad := d) in * by omega
-          end. eauto.
-        * indrep_n_extract; try omega. cancel.
-        * rewrite listmatch_updN_removeN. cancel. all: omega.
-        * erewrite upd_range_concat_hom_start_aligned by (eauto; omega). auto.
-        * rewrite natToWord_wordToNat. rewrite listmatch_updN_removeN by (eauto; omega). cancel.
-        * erewrite upd_range_concat_hom_start_aligned by (eauto; omega). auto.
-        * match goal with |- context [selN ?l ?ind ?d] =>
-            rewrite listmatch_extract with (b := l) (i := ind) (bd := d) in * by omega
+            rewrite listmatch_extract with (b := l) (i := ind) (bd := d) in *
           end. rewrite indrep_n_helper_length_piff in *.
           destruct_lifts.
           denote (length (selN _ _ _) = _) as Ha. rewrite Ha.
           omega.
-    + unfold indclear_from_aligned. fold indclear_from_aligned.
+          indrep_n_tree_bound.
+    + cbn [indclear_from_aligned].
       prestep. norml.
       pose proof listmatch_indrep_n_tree_forall_length (S indlvl) as H'.
-      simpl in H'. rewrite H' in *. destruct_lifts.
-      cancel; [> solve [hoare] |].
+      simpl in H'. rewrite H' in *.
+      denote (combine indbns fsl) as Hc; destruct_lift Hc.
+      cancel; [ solve [hoare] |].
       prestep. norml.
-      assert (start / (NIndirect ^ S (S indlvl)) < length l_part); simpl in *.
-        indrep_n_tree_bound. rewrite mult_comm. omega.
-      assert (start / (NIndirect ^ S (S indlvl)) < length indbns); simpl in *.
-        indrep_n_tree_bound. rewrite mult_comm. omega.
+      assert (start / (NIndirect ^ S (S indlvl)) < length l_part) by indrep_n_tree_bound.
+      assert (start / (NIndirect ^ S (S indlvl)) < length indbns) by indrep_n_tree_bound.
       cancel.
       step.
       {
         rewrite listmatch_extract in *.
+        erewrite selN_combine in * by auto. cbn [fst snd] in *.
         denote (# _ = _) as Ha. rewrite Ha in *.
         destruct_lifts.
         rewrite indrep_n_helper_0 in *.
+        destruct_lift H.
+        rewrite listmatch_indrep_n_tree_empty'' in *.
         destruct_lifts.
-        rewrite listmatch_repeat_l in *.
-        rewrite listpred_indrep_n_tree_0 in *. destruct_lifts.
         erewrite upd_range_concat_hom_start_aligned by (eauto; omega).
         denote (selN _ _ _ = _) as Hs. rewrite Hs.
-        denote (Forall _ _) as Hf. rewrite (concat_hom_repeat _ _ Hf) in *.
+        denote (Forall _ _) as Hf.
+        rewrite concat_repeat in *.
         rewrite upd_range_same by omega.
         erewrite selN_eq_updN_eq; eauto.
         omega.
+        indrep_n_tree_bound.
       }
       match goal with [|- context [selN ?L ?N] ] => 
-        rewrite listmatch_extract with (a := L) (i := N) in * by omega end.
+        rewrite listmatch_extract with (a := combine L _) (i := N) in * by indrep_n_tree_bound end.
       destruct_lifts.
+      rewrite combine_length_eq in * by omega.
       step.
-      { rewrite indrep_n_helper_valid by eauto. cancel. }
+      {
+        rewrite selN_combine by indrep_n_tree_bound; cbn [fst snd].
+        rewrite indrep_n_helper_valid by eauto. cancel.
+      }
       rewrite firstn_oob.
-      match goal with [H : context [listmatch _ ?l] |- context [?c = ?l] ] =>
-        rewrite listmatch_length_pimpl with (a := l) in H;
+      match goal with [H : context [listmatch _ (combine ?l _)] |- context [?c = ?l] ] =>
+        rewrite listmatch_length_pimpl with (a := combine l _) in H;
         rewrite indrep_n_helper_length_piff in H; destruct_lift H end.
-      step.
+      rewrite combine_length_eq in * by omega.
+      prestep. norm. cancel.
+      intuition auto.
+      pred_apply; cancel.
       {
         rewrite Nat.div_mul, Nat.div_0_l by auto. simpl in *.
         apply Nat.div_le_upper_bound; mult_nonzero. rewrite mult_comm.
         apply Nat.lt_le_incl. congruence.
+      }
+      indrep_n_tree_bound.
+      {
+        denote (snd (selN _ _ _)) as Hp.
+        rewrite selN_combine in Hp by indrep_n_tree_bound.
+        cbn [snd] in Hp.
+        pred_apply.
+        rewrite pred_fold_left_selN_removeN.
+        rewrite Hp.
+        cancel.
       }
       safestep.
       { rewrite Nat.div_0_l, Nat.div_mul by auto. cancel. }
@@ -1461,45 +1728,62 @@ Module BlockPtr (BPtr : BlockPtrSig).
         autorewrite with lists.
         apply Nat.lt_le_incl. congruence.
       }
-      step.
-      {
-        unfold IndRec.items_valid, IndSig.xparams_ok, IndSig.RAStart, IndSig.RALen.
-        rewrite mult_1_l. intuition.
-        match goal with [H : context [listmatch _ ?l] |- context [length ?l] ] =>
-          rewrite listmatch_length_pimpl with (a := l) in H; destruct_lift H;
-          substl (length l) end.
-        match goal with [H : context [concat ?l] |- context [length ?l] ] =>
-          apply f_equal with (f := @length _) in H; erewrite concat_hom_length in H; eauto end.
-        autorewrite with lists in *.
-        erewrite concat_hom_length in * by eauto.
-        rewrite upd_range_length in *.
-        rewrite Nat.mul_cancel_r in * by mult_nonzero. congruence.
-      }
-      step; clear IHindlvl.
-      - rewrite indrep_n_helper_0. cancel.
-        rewrite listmatch_updN_removeN. cancel.
-        rewrite indrep_n_helper_0. cancel.
-        all: omega.
-      - erewrite upd_range_concat_hom_start_aligned by (eauto; omega).
-        repeat f_equal.
-        denote (concat _ = _) as Hc. rewrite Hc.
-        denote (selN _ _ _ = _) as Hs. rewrite Hs.
-        rewrite concat_hom_upd_range by eauto. cbn -[Nat.div Nat.modulo].
-        autorewrite with lists. simpl.
-        rewrite mult_comm, <- Nat.div_mod; auto.
-      - rewrite natToWord_wordToNat. rewrite listmatch_updN_removeN. cancel.
-        all: omega.
-      - denote (concat _ = _) as Hc. rewrite Hc.
-        symmetry. erewrite upd_range_concat_hom_start_aligned by (eauto; mult_nonzero; omega).
-        rewrite concat_hom_upd_range; eauto.
-        rewrite upd_range_upd_range; eauto.
-        repeat f_equal; eauto.
-        rewrite mult_comm with (n := len / _), <- Nat.div_mod; auto.
+      autorewrite with lists; omega.
+      cancel.
+      prestep. norm. cancel.
+      rewrite selN_combine with (a := indbns) in * by eauto.
+      cbn [fst snd] in *.
+      intuition auto.
+      unfold IndRec.items_valid, IndSig.xparams_ok, IndSig.RAStart, IndSig.RALen.
+      rewrite mult_1_l. intuition.
+      rewrite upd_range_length in *.
+      indrep_n_tree_bound.
+      pred_apply; cancel.
+      pred_apply; cancel.
+      - step; clear IHindlvl.
+        5: match goal with |- context [removeN _ ?i] =>
+          erewrite pred_fold_left_selN_removeN with (l := updN fsl i (pred_fold_left fsl'0));
+          rewrite selN_updN_eq, removeN_updN by omega
+        end.
+        * rewrite indrep_n_helper_0. cancel.
+          rewrite combine_updN, listmatch_updN_removeN.
+          norm. cancel. eassign IFs'. rewrite indrep_n_helper_0. cancel.
+          intuition eauto. indrep_n_tree_bound.
+          denote (IFs' <=p=> emp) as Hf. rewrite Hf. split; cancel.
+          all: rewrite ?combine_length_eq; omega.
+        * erewrite upd_range_concat_hom_start_aligned by (eauto; omega).
+          repeat f_equal.
+          denote (concat _ = _) as Hc. rewrite Hc.
+          denote (selN _ _ _ = _) as Hs. rewrite Hs.
+          rewrite concat_hom_upd_range by eauto. cbn -[Nat.div Nat.modulo].
+          autorewrite with lists. simpl.
+          rewrite mult_comm, <- Nat.div_mod; auto.
+        * autorewrite with lists; auto.
+        * autorewrite with lists; omega.
+        * denote (indrep_n_helper _ _ 0) as Hi. rewrite indrep_n_helper_0 in Hi.
+          destruct_lift Hi. denote (IFs' <=p=> emp) as Hf. rewrite Hf. cancel.
+        * rewrite natToWord_wordToNat. rewrite combine_updN.
+          rewrite listmatch_updN_removeN. cancel. reflexivity.
+          indrep_n_tree_bound.
+          reflexivity.
+          all: rewrite ?combine_length_eq; omega.
+        * denote (concat _ = _) as Hc. rewrite Hc.
+          symmetry. erewrite upd_range_concat_hom_start_aligned by (eauto; mult_nonzero; omega).
+          rewrite concat_hom_upd_range; eauto.
+          rewrite upd_range_upd_range; eauto.
+          repeat f_equal; eauto.
+          rewrite mult_comm with (n := len / _), <- Nat.div_mod; auto.
+        * autorewrite with lists; auto.
+        * autorewrite with lists; auto.
+        * rewrite pred_fold_left_selN_removeN with (l := updN _ _ _).
+          rewrite selN_updN_eq, removeN_updN by omega. cancel.
       - cancel.
-      - unfold IndRec.Defs.item in *. simpl in *.
-        rewrite indrep_n_helper_length_piff in *. destruct_lifts. omega.
+      - cancel.
+      - cancel.
+      - indrep_n_tree_bound.
     Grab Existential Variables.
-    all : intros; solve [exact unit | exact nil | exact $ 0 | exact 0 | exact True].
+    all : intros; eauto.
+    all : try solve [exact unit | exact nil | exact $ 0 | exact 0 | exact True | exact ($0, emp) ].
   Qed.
 
   Hint Extern 1 ({{_}} Bind (indclear_from_aligned _ _ _ _ _ _ _) _) => apply indclear_from_aligned_ok : prog.
@@ -1534,20 +1818,24 @@ Module BlockPtr (BPtr : BlockPtrSig).
 
   Theorem indclear_to_aligned_ok : forall indlvl lxp bxp indbns start ms,
     let N := NIndirect ^ S indlvl in
-    {< F Fm m0 m l_part freelist,
+    {< F Fm Fs m0 sm m fsl l_part freelist,
     PRE:hm
-           LOG.rep lxp F (LOG.ActiveTxn m0 m) (BALLOCC.MSLog ms) hm *
-           [[[ m ::: (Fm * listmatch (fun ibn l => indrep_n_tree indlvl bxp (#ibn) l) indbns l_part
+           LOG.rep lxp F (LOG.ActiveTxn m0 m) (BALLOCC.MSLog ms) sm hm *
+           [[[ m ::: (Fm * listmatch (fun x l => indrep_n_tree indlvl bxp (snd x) #(fst x) l) (combine indbns fsl) l_part
                          * BALLOCC.rep bxp freelist ms) ]]] *
-           [[ start <= length (concat l_part) ]]
+           [[ (Fs * pred_fold_left fsl * BALLOCC.smrep freelist)%pred sm ]] *
+           [[ start <= length (concat l_part) ]] *
+           [[ length fsl = length indbns ]]
     POST:hm' RET:^(ms, indbns')
-           exists m' freelist' l_part', 
-           LOG.rep lxp F (LOG.ActiveTxn m0 m') (BALLOCC.MSLog ms) hm' *
-           [[[ m' ::: (Fm * listmatch (fun ibn l => indrep_n_tree indlvl bxp (#ibn) l) indbns' l_part'
+           exists m' freelist' fsl' l_part',
+           LOG.rep lxp F (LOG.ActiveTxn m0 m') (BALLOCC.MSLog ms) sm hm' *
+           [[[ m' ::: (Fm * listmatch (fun x l => indrep_n_tree indlvl bxp (snd x) #(fst x) l) (combine indbns' fsl') l_part'
                           * BALLOCC.rep bxp freelist' ms) ]]] *
            [[ concat (l_part') = upd_range (concat l_part) start (roundup start N - start) $0 ]] *
-           [[ incl freelist freelist' ]]
-    CRASH:hm'  LOG.intact lxp F m0 hm'
+           [[ incl freelist freelist' ]] *
+           [[ (Fs * pred_fold_left fsl' * BALLOCC.smrep freelist')%pred sm ]] *
+           [[ length fsl' = length indbns' ]]
+    CRASH:hm'  LOG.intact lxp F m0 sm hm'
     >} indclear_to_aligned indlvl lxp bxp indbns start ms.
   Proof.
     induction indlvl.
@@ -1558,8 +1846,9 @@ Module BlockPtr (BPtr : BlockPtrSig).
         unfold roundup. rewrite divup_eq_div by auto.
         rewrite mul_div by auto. autorewrite with core lists. auto.
       }
-      rewrite (listmatch_indrep_n_tree_forall_length 0) in *.
-      destruct_lifts. rewrite mult_1_r in *.
+      denote indrep_n_helper as Hi.
+      setoid_rewrite (listmatch_indrep_n_tree_forall_length 0) in Hi.
+      destruct_lift Hi. rewrite mult_1_r in *.
       rewrite listmatch_length_pimpl in *. destruct_lifts.
       prestep. norml.
       assert (start / NIndirect < length l_part).
@@ -1567,49 +1856,90 @@ Module BlockPtr (BPtr : BlockPtrSig).
         apply Nat.div_lt_upper_bound; auto. rewrite mult_comm.
         edestruct le_lt_eq_dec; [> | eauto |]; eauto.
         subst. rewrite Nat.mod_mul in * by auto. intuition.
-      step.
-      {
+      cancel.
+      prestep. norm. cancel.
+      intuition auto.
+      Focus 2. {
         rewrite roundup_eq, minus_plus by auto.
         rewrite listmatch_extract in *.
-        denote (# _ = _) as Hn. rewrite Hn in *. rewrite indrep_n_helper_0 in *.
-        destruct_lifts. erewrite upd_range_concat_hom_small; eauto.
-        erewrite selN_eq_updN_eq. auto.
-        denote (selN _ _ _ = _) as Hs. rewrite Hs.
+        erewrite <- upd_range_concat_hom_small; eauto.
         all : autorewrite with core lists; auto with *; eauto.
         rewrite <- roundup_eq by auto.
         erewrite concat_hom_length in * by eauto.
         apply roundup_le. omega.
+        eassign (start / NIndirect).
+        rewrite min_l by omega.
+        rewrite combine_length_eq in *; omega.
+      } Unfocus.
+      {
+        pred_apply; cancel.
+        erewrite <- updN_selN_eq with (l := combine _ _) at 2.
+        rewrite listmatch_updN_removeN.
+        indrep_n_extract.
+        repeat rewrite selN_combine by auto. cbn [fst snd].
+        denote (# _ = _) as Hn. repeat rewrite Hn. rewrite indrep_n_helper_0 in *.
+        cancel. rewrite indrep_n_helper_0.
+        (* same bug *)
+        do 2 intro; apply sep_star_lift_apply'; cbv [lift_empty]; intuition auto.
+        denote (_ = repeat _ _) as Hl. rewrite Hl.
+        apply upd_range_same.
+        eauto.
+        all: omega.
       }
-      indrep_n_extract. rewrite indrep_n_helper_valid by eassumption. cancel.
+      auto.
+      pred_apply; cancel.
+      omega.
+      step.
+      indrep_n_extract. rewrite indrep_n_helper_valid by eauto. cancel.
       rewrite firstn_oob.
-      hoare.
+      prestep. norm. cancel.
+      intuition auto.
       - match goal with [|- context [selN ?L ?N ?d] ] =>
-          rewrite listmatch_extract with (a := L) (i := N) (ad := d) in * by omega
-        end. eauto.
+          erewrite listmatch_extract with (a := combine L _) (i := N) (ad := (d, _)) in * by omega
+        end. rewrite selN_combine in * by auto. cbn [fst snd] in *. eauto.
       - match goal with [|- context [selN ?L ?N ?d] ] =>
-          rewrite listmatch_extract with (a := L) (i := N) (ad := d) in * by omega
-        end. eauto.
-      - indrep_n_extract. cancel.
-      - rewrite listmatch_updN_removeN. cancel. all: omega.
-      - rewrite roundup_eq by auto. rewrite minus_plus.
-        erewrite upd_range_concat_hom_small; eauto.
-        all : autorewrite with core; eauto.
-        rewrite <- roundup_eq by auto.
-        erewrite concat_hom_length in *; eauto.
-      - rewrite natToWord_wordToNat. rewrite listmatch_updN_removeN by (eauto; omega). cancel.
-      - rewrite roundup_eq by auto. rewrite minus_plus.
-        erewrite upd_range_concat_hom_small; eauto.
-        rewrite <- roundup_eq by auto.
-        erewrite concat_hom_length in * by eauto. auto.
-        rewrite le_plus_minus_r; auto.
+          erewrite listmatch_extract with (a := combine L _) (i := N) (ad := (d, _)) in * by omega
+        end. rewrite selN_combine in * by auto. cbn [fst snd] in *.
+        rewrite indrep_n_helper_items_valid in * by eauto; destruct_lifts.
+        unfold IndRec.items_valid in *; intuition.
+        autorewrite with lists; eauto.
+      - pred_apply. indrep_n_extract. cancel.
+      - pred_apply. rewrite pred_fold_left_selN_removeN with (i := start/NIndirect) (l := fsl).
+        cancel. instantiate (1 := emp). cancel.
+      - prestep; norm; try cancel.
+        all: intuition auto.
+        * pred_apply. erewrite combine_updN. rewrite listmatch_updN_removeN. cancel. all: omega.
+        * rewrite roundup_eq by auto. rewrite minus_plus.
+          erewrite upd_range_concat_hom_small; eauto.
+          all : autorewrite with core; eauto.
+          rewrite <- roundup_eq by auto.
+          erewrite concat_hom_length in *; eauto.
+        * auto.
+        * rewrite pred_fold_left_updN_removeN by (rewrite combine_length_eq in *; omega).
+          pred_apply; cancel.
+        * autorewrite with lists; auto.
+        * rewrite natToWord_wordToNat. rewrite combine_updN.
+          rewrite listmatch_updN_removeN. pred_apply; cancel.
+          all: rewrite ?combine_length_eq; try omega; indrep_n_tree_bound.
+          rewrite mult_comm; eauto using div_lt_mul_lt.
+        * rewrite roundup_eq by auto. rewrite minus_plus.
+          erewrite upd_range_concat_hom_small; eauto.
+          rewrite <- roundup_eq by auto.
+          erewrite concat_hom_length in * by eauto. auto.
+          rewrite le_plus_minus_r; auto.
+        * auto.
+        * rewrite pred_fold_left_updN_removeN by (rewrite combine_length_eq in *; omega).
+          pred_apply; cancel.
+        * autorewrite with lists; auto.
+      - cancel.
       - match goal with [|- context [selN ?L ?N ?d] ] =>
           rewrite listmatch_extract with (b := L) (i := N) (bd := d) in * by omega
         end. rewrite indrep_n_helper_length_piff in *.
         destruct_lifts. autorewrite with core. apply Nat.eq_le_incl. assumption.
-    + unfold indclear_to_aligned. fold indclear_to_aligned.
+    + cbn [indclear_to_aligned].
       prestep. norml.
       pose proof listmatch_indrep_n_tree_forall_length (S indlvl) as H'.
-      simpl in H'. rewrite H' in *. destruct_lifts.
+      simpl in H'. match goal with H: _ |- _ => rewrite H' in H; destruct_lift H end.
       cancel. hoare.
       {
         unfold roundup. rewrite divup_eq_div by auto. rewrite mul_div by mult_nonzero.
@@ -1622,37 +1952,56 @@ Module BlockPtr (BPtr : BlockPtrSig).
         apply Nat.div_lt_upper_bound; auto. rewrite mult_comm.
         edestruct le_lt_eq_dec; [> | eauto |]; eauto.
         subst. rewrite Nat.mod_mul in * by auto. intuition.
-      cancel. step.
+      cancel. prestep. norm. cancel.
+      instantiate (1 := updN _ _ _). intuition auto.
+      {
+        erewrite <- updN_selN_eq with (l := indbns) at 1.
+        rewrite combine_updN. rewrite listmatch_updN_removeN.
+        denote (# _ = 0) as Hn. cbn [fst snd].
+        pred_apply. rewrite listmatch_extract. rewrite selN_combine.
+        cbn [fst snd]. repeat rewrite Hn. cancel. reflexivity.
+        all: eauto; omega.
+      }
       {
         rewrite roundup_eq, minus_plus by auto.
         rewrite listmatch_extract in *. destruct_lifts.
         erewrite upd_range_concat_hom_small; eauto.
+        erewrite selN_combine in *. cbn [fst snd] in *.
         denote (# _ = 0) as Hn. rewrite Hn in *.
         rewrite indrep_n_helper_0 in *. destruct_lifts.
-        rewrite listmatch_repeat_l in *.
-        rewrite listpred_indrep_n_tree_0 in *. destruct_lifts.
-        erewrite selN_eq_updN_eq. auto.
-        denote (selN _ _ _ = _) as Hs. rewrite Hs.
-        erewrite concat_hom_repeat in * by eauto.
-        rewrite upd_range_same by omega. eauto.
-        all : autorewrite with core; mult_nonzero; auto with *.
+        rewrite listmatch_indrep_n_tree_empty'' in *. destruct_lifts.
+        do 2 f_equal.
+        denote (selN _ _ _ = _) as Hs. repeat rewrite Hs.
+        erewrite concat_hom_repeat by (auto using Forall_repeat).
+        rewrite upd_range_same; auto.
+        all: try omega; mult_nonzero.
         erewrite concat_hom_length in * by eauto.
         rewrite <- roundup_eq; auto.
+        indrep_n_tree_bound.
       }
+      auto.
+      rewrite updN_selN_eq. auto.
+      autorewrite with lists; auto.
       match goal with [|- context [selN ?L ?N ?d] ] =>
-        rewrite listmatch_extract with (a := L) (i := N) (ad := d) in * by omega
+        rewrite listmatch_extract with (a := combine L _) (i := N) (ad := (d, emp)) in * by omega
       end. simpl in *. destruct_lifts.
+      rewrite selN_combine in * by omega; cbn [fst snd] in *.
       step.
       { rewrite indrep_n_helper_valid by eauto. cancel. }
       rewrite firstn_oob.
-      match goal with [H : context [listmatch _ ?l] |- context [?c = ?l] ] =>
-        rewrite listmatch_length_pimpl with (a := l) in H;
+      match goal with [H : context [listmatch _ (combine ?l _)] |- context [?c = ?l] ] =>
+        rewrite listmatch_length_pimpl with (a := combine l _) in H;
         rewrite indrep_n_helper_length_piff in H; destruct_lift H end.
-      step.
+      prestep. norm. cancel.
+      intuition auto.
+      pred_apply; cancel.
+      pred_apply. rewrite pred_fold_left_selN_removeN with (l := fsl).
+      denote (selN fsl) as Hs. rewrite Hs. cancel.
       {
         erewrite concat_hom_length by eauto.
-        eapply le_trans; [> | apply mult_le_compat_r]. eauto. omega.
+        eapply le_trans; [> | apply mult_le_compat_r]. eauto. indrep_n_tree_bound.
       }
+      omega.
       safestep.
       {
         unfold roundup. rewrite <- Nat.mul_sub_distr_r. repeat rewrite Nat.div_mul by auto.
@@ -1661,46 +2010,68 @@ Module BlockPtr (BPtr : BlockPtrSig).
           apply f_equal with (f := @length _) in H; erewrite concat_hom_length in H; eauto end.
         rewrite upd_range_length in *; autorewrite with core; auto with *.
         erewrite concat_hom_length in * by eauto.
-        rewrite Nat.mul_cancel_r in *; mult_nonzero. omega.
+        rewrite Nat.mul_cancel_r in *; mult_nonzero.
+        rewrite combine_length_eq in * by omega. omega.
         apply divup_le. rewrite mult_comm. eauto.
       }
-      step.
+      prestep. norm. cancel. intuition idtac.
+      auto.
       {
         unfold IndRec.items_valid, IndSig.xparams_ok, IndSig.RAStart, IndSig.RALen.
         rewrite mult_1_l.
-        match goal with [H : context [listmatch _ ?l] |- context [length (upd_range ?l _ _ _)] ] =>
-          rewrite listmatch_length_pimpl with (a := l) in H; destruct_lift H end.
+        match goal with [H : context [listmatch _ (combine ?l _)] |- context [length (upd_range ?l _ _ _)] ] =>
+          rewrite listmatch_length_pimpl with (a := (combine l _)) in H; destruct_lift H end.
         denote (concat _ = upd_range _ _ _ _) as Hc.
         apply f_equal with (f := @length _) in Hc.
-        erewrite concat_hom_length in Hc by eauto.
+        rewrite combine_length_eq in * by omega.
+        erewrite concat_hom_length in Hc; eauto.
         autorewrite with lists in *.
         erewrite concat_hom_length in * by eauto.
         rewrite Nat.mul_cancel_r in *; mult_nonzero.
         intuition; omega.
       }
+      pred_apply; cancel.
+      pred_apply; cancel.
       step; clear IHindlvl.
       - rewrite indrep_n_helper_0. cancel.
-        rewrite listmatch_updN_removeN. cancel. rewrite indrep_n_helper_0. cancel.
+        rewrite combine_updN, listmatch_updN_removeN.
+        norm. cancel. rewrite indrep_n_helper_0'. cancel.
         unfold roundup. rewrite <- Nat.mul_sub_distr_r.
-        repeat rewrite Nat.div_mul by auto. assumption.
+        repeat rewrite Nat.div_mul by auto.
+        denote (upd_range _ _ _) as Hu. rewrite Hu.
+        cancel. reflexivity.
+        intuition eauto.
         all : omega.
       - rewrite roundup_eq with (a := start) by mult_nonzero.
         rewrite minus_plus.
-        unfold roundup. rewrite <- Nat.mul_sub_distr_r. repeat rewrite Nat.div_mul by mult_nonzero.
         eapply indclear_upd_range_helper_1; eauto.
-        erewrite concat_hom_length by eauto. congruence.
+        erewrite concat_hom_length by eauto.
+        rewrite combine_length_eq2 in * by omega. congruence.
+      - rewrite pred_fold_left_updN_removeN.
+        rewrite indrep_n_helper_0 with (Fs := IFs') in *.
+        denote (IFs' <=p=> emp) as Hf; destruct_lift Hf.
+        psubst. cancel.
+        rewrite combine_length_eq in * by omega. omega.
+      - autorewrite with lists; auto.
       - rewrite natToWord_wordToNat.
         unfold roundup. rewrite <- Nat.mul_sub_distr_r. repeat rewrite Nat.div_mul by auto.
-        rewrite listmatch_updN_removeN. cancel.
+        rewrite combine_updN.
+        rewrite listmatch_updN_removeN. cancel; eauto.
         all : omega.
       - erewrite indclear_upd_range_helper_1; eauto.
         f_equal. rewrite roundup_eq by auto. omega.
-        erewrite concat_hom_length by eauto. congruence.
+        erewrite concat_hom_length by eauto.
+        rewrite combine_length_eq in * by omega. congruence.
+      - rewrite pred_fold_left_updN_removeN. cancel.
+        rewrite combine_length_eq in * by omega. omega.
+      - autorewrite with lists; auto.
+      - cancel.
+      - cancel.
       - cancel.
       - rewrite indrep_n_helper_length_piff in *. destruct_lifts.
         unfold IndRec.Defs.item in *. simpl in *. omega.
     Unshelve.
-    all : intros; try solve [exact unit | exact nil | exact $0 | constructor].
+    all : intros; try solve [exact unit | exact nil | exact $0 | exact emp | exact ($0, emp) | constructor].
   Qed.
 
   Local Hint Extern 1 ({{_}} Bind (indclear_to_aligned _ _ _ _ _ _) _) => apply indclear_to_aligned_ok : prog.
@@ -1718,27 +2089,32 @@ Module BlockPtr (BPtr : BlockPtrSig).
 
   Theorem indclear_multiple_blocks_ok : forall indlvl lxp bxp indbns start len ms,
     let N := NIndirect ^ S indlvl in
-    {< F Fm m0 m l_part freelist,
+    {< F Fm Fs m0 sm m l_part freelist fsl,
     PRE:hm
-           LOG.rep lxp F (LOG.ActiveTxn m0 m) (BALLOCC.MSLog ms) hm *
-           [[[ m ::: (Fm * listmatch (fun ibn l => indrep_n_tree indlvl bxp (#ibn) l) indbns l_part
+           LOG.rep lxp F (LOG.ActiveTxn m0 m) (BALLOCC.MSLog ms) sm hm *
+           [[[ m ::: (Fm * listmatch (fun x l => indrep_n_tree indlvl bxp (snd x) #(fst x) l) (combine indbns fsl) l_part
                          * BALLOCC.rep bxp freelist ms) ]]] *
            [[ start <= length (concat l_part) ]] * [[ (N - start mod N) < len ]] *
-           [[ start + len <= length (concat l_part) ]]
+           [[ start + len <= length (concat l_part) ]] *
+           [[ (Fs * pred_fold_left fsl * BALLOCC.smrep freelist)%pred sm ]] *
+           [[ length indbns = length fsl ]]
     POST:hm' RET:^(ms, indbns')
-           exists m' freelist' l_part', 
-           LOG.rep lxp F (LOG.ActiveTxn m0 m') (BALLOCC.MSLog ms) hm' *
-           [[[ m' ::: (Fm * listmatch (fun ibn l => indrep_n_tree indlvl bxp (#ibn) l) indbns' l_part'
+           exists m' freelist' l_part' fsl',
+           LOG.rep lxp F (LOG.ActiveTxn m0 m') (BALLOCC.MSLog ms) sm hm' *
+           [[[ m' ::: (Fm * listmatch (fun x l => indrep_n_tree indlvl bxp (snd x) #(fst x) l) (combine indbns' fsl') l_part'
                           * BALLOCC.rep bxp freelist' ms) ]]] *
            [[ concat (l_part') = upd_range (concat l_part) start len $0 ]] *
+           [[ (Fs * pred_fold_left fsl' * BALLOCC.smrep freelist')%pred sm ]] *
+           [[ length indbns' = length fsl' ]] *
            [[ incl freelist freelist' ]]
-    CRASH:hm'  LOG.intact lxp F m0 hm'
+    CRASH:hm'  LOG.intact lxp F m0 sm hm'
     >} indclear_multiple_blocks indlvl lxp bxp indbns start len ms.
   Proof.
     intros. subst N.
     unfold indclear_multiple_blocks.
-    hoare.
-    + repeat rewrite Nat.div_mul by mult_nonzero.
+    step.
+    step.
+    { repeat rewrite Nat.div_mul by mult_nonzero.
       eapply le_trans. apply div_add_distr_le.
       denote (concat _ = _) as Hc.
       apply f_equal with (f := @length _) in Hc.
@@ -1751,8 +2127,11 @@ Module BlockPtr (BPtr : BlockPtrSig).
         autorewrite with core. congruence.
       - rewrite roundup_eq by auto. rewrite minus_plus.
         rewrite <- plus_assoc. autorewrite with core; solve [congruence | omega].
-    + autorewrite with core; auto.
-    + repeat rewrite Nat.div_mul by auto. cancel.
+    }
+    { autorewrite with core; auto. }
+    prestep. norm. cancel.
+    intuition auto.
+    + pred_apply. repeat rewrite Nat.div_mul by auto. cancel.
     + erewrite concat_hom_length by auto. autorewrite with lists.
       rewrite mult_comm with (m := _ * _ ^ _).
       rewrite <- plus_assoc, <- Nat.div_mod by auto.
@@ -1767,7 +2146,10 @@ Module BlockPtr (BPtr : BlockPtrSig).
       - rewrite roundup_eq by auto. rewrite minus_plus.
         rewrite <- plus_assoc. autorewrite with core; solve [congruence | omega].
     + autorewrite with core. auto.
-    + rewrite concat_hom_upd_range in * by eauto.
+    + autorewrite with lists in *. omega.
+    + pred_apply; cancel.
+    + step.
+      rewrite concat_hom_upd_range in * by eauto.
       set (N := _ * _ ^ _) in *.
       rewrite le_plus_minus_r in * by auto.
       rewrite roundup_round in *.
@@ -1780,6 +2162,7 @@ Module BlockPtr (BPtr : BlockPtrSig).
       - unfold roundup. rewrite divup_eq_div by auto. rewrite mul_div by mult_nonzero. omega.
       - rewrite roundup_eq by mult_nonzero. autorewrite with core; omega.
       - auto.
+    + cancel.
     Unshelve.
       all : solve [exact unit | exact nil].
   Qed.
@@ -1812,47 +2195,54 @@ Module BlockPtr (BPtr : BlockPtrSig).
     }.
 
   Theorem indclear_ok : forall indlvl lxp bxp ir start len ms,
-    {< F Fm m0 m l freelist,
+    {< F Fm Fs m0 sm m l freelist IFs,
     PRE:hm
-           LOG.rep lxp F (LOG.ActiveTxn m0 m) (BALLOCC.MSLog ms) hm *
-           [[[ m ::: (Fm * indrep_n_tree indlvl bxp ir l * 
+           LOG.rep lxp F (LOG.ActiveTxn m0 m) (BALLOCC.MSLog ms) sm hm *
+           [[[ m ::: (Fm * indrep_n_tree indlvl bxp IFs ir l *
             BALLOCC.rep bxp freelist ms) ]]] *
-           [[ start + len <= length l ]]
+           [[ start + len <= length l ]] *
+           [[ (Fs * IFs * BALLOCC.smrep freelist)%pred sm ]]
     POST:hm' RET:^(ms, ir')
-           exists m' freelist' l', 
-           LOG.rep lxp F (LOG.ActiveTxn m0 m') (BALLOCC.MSLog ms) hm' *
-           [[[ m' ::: (Fm * indrep_n_tree indlvl bxp ir' l' * 
+           exists m' freelist' l' IFs',
+           LOG.rep lxp F (LOG.ActiveTxn m0 m') (BALLOCC.MSLog ms) sm hm' *
+           [[[ m' ::: (Fm * indrep_n_tree indlvl bxp IFs' ir' l' *
               BALLOCC.rep bxp freelist' ms) ]]] *
            [[ incl freelist freelist' ]] * [[ l' = upd_range l start len $0 ]] *
+           [[ (Fs * IFs' * BALLOCC.smrep freelist')%pred sm ]] *
            ([[ ir = ir' ]] \/ [[ ir' = 0 ]])
-    CRASH:hm'  LOG.intact lxp F m0 hm'
+    CRASH:hm'  LOG.intact lxp F m0 sm hm'
     >} indclear indlvl lxp bxp ir start len ms.
     Proof.
       induction indlvl.
-      + simpl. hoare.
-        rewrite indrep_n_helper_length_piff, indrep_n_helper_0 in *. destruct_lifts.
-        rewrite upd_range_same. auto.
-        rewrite indrep_n_helper_valid by auto. cancel.
-        all : match goal with H : _ |- _ =>
-          rewrite indrep_n_helper_length_piff in H;
-          destruct_lift H;
-          unfold IndRec.Defs.item in *; simpl in *; rewrite firstn_oob by omega;
-          try cancel; auto
-        end.
-      + simpl.
+      + cbn -[Nat.div].
+        prestep. norml.
+        denote indrep_n_helper as Hi.
+        rewrite indrep_n_helper_length_piff in Hi; destruct_lift Hi.
+        step.
+        rewrite indrep_n_helper_0 in *. destruct_lifts.
+        autorewrite with lists; auto.
+        - hoare.
+        - step.
+          rewrite indrep_n_helper_valid by auto; cancel.
+          rewrite firstn_oob by indrep_n_tree_bound.
+          hoare.
+      + cbn [indclear].
         step. step.
         {
-          rewrite indrep_n_helper_0 in *. destruct_lifts.
-          rewrite listmatch_repeat_l in *. rewrite listpred_indrep_n_tree_0 in *.
-          destruct_lifts. erewrite concat_hom_repeat by eauto.
+          denote indrep_n_helper as Hi.
+          rewrite indrep_n_helper_0 in Hi. destruct_lift Hi.
+          rewrite listmatch_indrep_n_tree_empty'' in H.
+          destruct_lift H.
+          erewrite concat_hom_repeat by eauto using Forall_repeat.
           autorewrite with lists. reflexivity.
+          rewrite repeat_length in *; auto.
         }
         step. solve [step].
         step.
         { rewrite indrep_n_helper_valid by auto. cancel. }
         rewrite indrep_n_helper_length_piff in *. destruct_lifts.
         unfold IndRec.Defs.item in *; simpl in *.
-        rewrite firstn_oob by omega.
+        rewrite firstn_oob by indrep_n_tree_bound.
         step.
         - safestep.
           indrep_n_extract; solve [cancel | indrep_n_tree_bound].
@@ -1862,68 +2252,98 @@ Module BlockPtr (BPtr : BlockPtrSig).
           indrep_n_tree_extract_lengths.
           denote (length _ = _) as Hl. rewrite Hl. omega.
           indrep_n_tree_bound.
+          psubst.
+          match goal with |- context [selN _ ?n] =>
+            rewrite pred_fold_left_selN_removeN with (i := n) end. cancel.
+          instantiate (1 := emp). cancel.
           safestep; rewrite ?natToWord_wordToNat, ?updN_selN_eq.
-          eauto.
-          * prestep. norm. cancel. or_r. cancel.
-            rewrite indrep_n_helper_0 in *.
-            destruct_lifts.
-            intuition auto.
-            pred_apply. norm; intuition eauto.
-            instantiate (iblocks := updN _ _ _). cancel.
-            match goal with |- context [removeN ?l ?i_] =>
-              rewrite listmatch_updN_removeN with (a := l) (i := i_)
-            end. cancel.
-            rewrite updN_selN_eq.
-            rewrite indrep_n_helper_0; cancel.
-            indrep_n_tree_bound.
-            indrep_n_tree_bound.
-            erewrite upd_range_concat_hom_small by (eauto; mult_nonzero; omega). auto.
-            auto.
-            cancel. or_l. cancel.
+          * prestep. norm. cancel. cancel.
+            assert (dummy = repeat $0 NIndirect).
+            rewrite indrep_n_helper_0 in H8. destruct_lift H8. auto.
+            subst.
+            rewrite repeat_selN' in *.
+            {
+              intuition auto. pred_apply. cancel.
+              erewrite listmatch_isolate with (a := combine _ _).
+              erewrite combine_updN_r with (x := IFs').
+              rewrite removeN_updN, selN_updN_eq.
+              cbn [fst snd].
+              rewrite repeat_selN'. rewrite removeN_updN, selN_updN_eq.
+              cancel.
+              all: autorewrite with lists; auto.
+              indrep_n_tree_bound.
+              indrep_n_tree_bound.
+              indrep_n_tree_bound.
+              indrep_n_tree_bound.
+              indrep_n_tree_bound.
+              eauto.
+              erewrite upd_range_concat_hom_small by (eauto; mult_nonzero; omega). auto.
+              pred_apply.
+              rewrite pred_fold_left_updN_removeN.
+              cancel.
+              rewrite repeat_length in *; substl (length dummy1).
+              indrep_n_tree_bound.
+            }
+            repeat cancel.
             intuition auto.
             pred_apply. norm; intuition.
-            instantiate (iblocks := updN _ _ _). cancel.
-            match goal with |- context [removeN ?l ?i_] =>
-              rewrite listmatch_updN_removeN with (a := l) (i := i_)
-            end. cancel.
+            rewrite combine_updN. cancel.
+            rewrite listmatch_updN_removeN. cancel.
             rewrite updN_selN_eq. cancel.
             indrep_n_tree_bound.
             indrep_n_tree_bound.
+            autorewrite with lists; omega.
+            eauto.
             erewrite upd_range_concat_hom_small by (eauto; mult_nonzero; omega). auto.
             auto.
+            rewrite pred_fold_left_updN_removeN.
+            pred_apply; cancel.
+            replace (length dummy1) with NIndirect by indrep_n_tree_bound.
+            indrep_n_tree_bound.
           * cancel.
           * prestep. norm. cancel. cancel. intuition auto.
             pred_apply. norm; intuition.
-            instantiate (iblocks := updN _ _ _). cancel.
+            rewrite combine_updN. cancel.
             rewrite listmatch_updN_removeN. repeat rewrite indrep_n_helper_0. cancel.
             indrep_n_tree_bound.
             indrep_n_tree_bound.
+            autorewrite with lists; auto.
+            eauto.
             erewrite upd_range_concat_hom_small by (eauto; mult_nonzero; omega).
             auto.
             auto.
-            cancel. cancel.
+            rewrite pred_fold_left_updN_removeN by (substl (length dummy1); indrep_n_tree_bound).
+            pred_apply; cancel.
+            repeat cancel.
             intuition auto.
             pred_apply. norm; intuition.
-            instantiate (iblocks := updN _ _ _). cancel.
+            rewrite combine_updN. cancel.
             rewrite listmatch_updN_removeN. repeat rewrite indrep_n_helper_0. cancel.
             indrep_n_tree_bound.
             indrep_n_tree_bound.
+            autorewrite with lists; auto.
+            eauto.
             erewrite upd_range_concat_hom_small by (eauto; mult_nonzero; omega).
             auto.
             auto.
+            rewrite pred_fold_left_updN_removeN by (substl (length dummy1); indrep_n_tree_bound).
+            pred_apply; cancel.
           * cancel.
           * cancel.
-      - hoare.
+      - step.
+        psubst. cancel.
+        step.
         unfold IndRec.items_valid, IndSig.xparams_ok, IndSig.RAStart, IndSig.RALen, Rec.well_formed.
         simpl. intuition auto.
-        match goal with [H : concat _ = _|- _] => apply f_equal with (f := @length _) in H end.
         indrep_n_tree_bound.
+        match goal with [H : concat _ = _|- _] => apply f_equal with (f := @length _) in H end.
         autorewrite with lists in *.
         indrep_n_tree_bound.
-        rewrite Nat.mul_cancel_r in * by mult_nonzero.
-        unfold IndRec.Defs.item. simpl. omega.
+        rewrite Nat.mul_cancel_r in *; auto.
+        step.
     Grab Existential Variables.
-    all : eauto; exact $0.
+    all : eauto.
+    all: try constructor; solve [exact $0 | exact emp].
   Qed.
 
   Local Hint Extern 1 ({{_}} Bind (indclear _ _ _ _ _ _ _ ) _) => apply indclear_ok : prog.
@@ -2162,41 +2582,43 @@ Module BlockPtr (BPtr : BlockPtrSig).
 
   Opaque indrep_n_tree.
 
-  Definition indrep bxp ir (indlist : list waddr) :=
-    ( indrep_n_tree 0 bxp (IRIndPtr ir) (firstn NIndirect indlist) *
-      indrep_n_tree 1 bxp (IRDindPtr ir) (firstn (NIndirect ^ 2) (skipn NIndirect indlist)) *
-      indrep_n_tree 2 bxp (IRTindPtr ir) (skipn (NIndirect + NIndirect ^ 2) indlist)
+  Definition indrep bxp Fs ir (indlist : list waddr) :=
+    (exists Fs0 Fs1 Fs2, [[ Fs <=p=> Fs0 * Fs1 * Fs2 ]] *
+      indrep_n_tree 0 bxp Fs0 (IRIndPtr ir) (firstn NIndirect indlist) *
+      indrep_n_tree 1 bxp Fs1 (IRDindPtr ir) (firstn (NIndirect ^ 2) (skipn NIndirect indlist)) *
+      indrep_n_tree 2 bxp Fs2 (IRTindPtr ir) (skipn (NIndirect + NIndirect ^ 2) indlist)
     )%pred.
 
-  Definition rep bxp (ir : irec) (l : list waddr) :=
+  Definition rep bxp Fs (ir : irec) (l : list waddr) :=
     ( [[ length l = (IRLen ir) /\ length l <= NBlocks ]] *
       [[ length (IRBlocks ir) = NDirect ]] *
-      exists indlist, indrep bxp ir indlist *
+      exists indlist, indrep bxp Fs ir indlist *
       [[ l = firstn (length l) ((IRBlocks ir) ++ indlist) ]] *
       [[ list_same $0 (skipn (length l) ((IRBlocks ir) ++ indlist)) ]] )%pred.
 
-  Definition rep_direct bxp (ir : irec) (l : list waddr) : @pred _ addr_eq_dec valuset :=
+  Definition rep_direct bxp Fs (ir : irec) (l : list waddr) : @pred _ addr_eq_dec valuset :=
     ( [[ length l = (IRLen ir) /\ length l <= NBlocks /\ length l <= NDirect ]] *
       [[ length (IRBlocks ir) = NDirect ]] *
-      exists indlist, indrep bxp ir indlist *
+      exists indlist, indrep bxp Fs ir indlist *
       [[ l = firstn (length l) (IRBlocks ir) ]] *
       [[ list_same $0 (skipn (length l) (IRBlocks ir)) ]] *
       [[ list_same $0 indlist ]] )%pred.
 
-  Definition rep_indirect bxp (ir : irec) (l : list waddr) :=
+  Definition rep_indirect bxp Fs (ir : irec) (l : list waddr) :=
     ( [[ length l = (IRLen ir) /\ length l <= NBlocks /\ length l > NDirect ]] *
       [[ length (IRBlocks ir) = NDirect ]] *
-      exists indlist, indrep bxp ir indlist *
+      exists indlist, indrep bxp Fs ir indlist *
       [[ l = (IRBlocks ir) ++ firstn (length l - NDirect) indlist ]] *
       [[ list_same $0 (skipn (length l - NDirect) indlist) ]] )%pred.
+
 
   Hint Resolve list_same_app_l.
   Hint Resolve list_same_app_r.
   Hint Resolve list_same_app_both.
 
-  Lemma rep_piff_direct : forall bxp ir l,
+  Lemma rep_piff_direct : forall bxp Fs ir l,
     length l <= NDirect ->
-    rep bxp ir l <=p=> rep_direct bxp ir l.
+    rep bxp Fs ir l <=p=> rep_direct bxp Fs ir l.
   Proof.
     intros. unfold rep, rep_direct. split; cancel.
     - rewrite firstn_app_l in * by omega; auto.
@@ -2206,9 +2628,9 @@ Module BlockPtr (BPtr : BlockPtrSig).
     - rewrite skipn_app_l by omega; eauto.
   Qed.
 
-  Lemma rep_piff_indirect : forall bxp ir l,
+  Lemma rep_piff_indirect : forall bxp Fs ir l,
     length l > NDirect ->
-    rep bxp ir l <=p=> rep_indirect bxp ir l.
+    rep bxp Fs ir l <=p=> rep_indirect Fs bxp ir l.
   Proof.
     unfold rep, rep_indirect; intros; split; cancel; try omega.
     - rewrite <- firstn_app_r; setoid_rewrite H3.
@@ -2219,8 +2641,8 @@ Module BlockPtr (BPtr : BlockPtrSig).
     - rewrite skipn_app_r_ge by omega. congruence.
   Qed.
 
-  Lemma rep_selN_direct_ok : forall F bxp ir l m off,
-    (F * rep bxp ir l)%pred m ->
+  Lemma rep_selN_direct_ok : forall F bxp Fs ir l m off,
+    (F * rep bxp Fs ir l)%pred m ->
     off < NDirect ->
     off < length l ->
     selN (IRBlocks ir) off $0 = selN l off $0.
@@ -2231,7 +2653,8 @@ Module BlockPtr (BPtr : BlockPtrSig).
     rewrite selN_app1 by omega; auto.
   Qed.
 
-  Theorem indrep_length_pimpl : forall bxp ir l, indrep bxp ir l <=p=> indrep bxp ir l * [[ length l = NBlocks - NDirect ]].
+  Theorem indrep_length_pimpl : forall bxp Fs ir l,
+    indrep bxp Fs ir l <=p=> indrep bxp Fs ir l * [[ length l = NBlocks - NDirect ]].
   Proof.
     intros.
     unfold indrep.
@@ -2244,9 +2667,9 @@ Module BlockPtr (BPtr : BlockPtrSig).
     f_equal; eauto. rewrite skipn_skipn'. auto.
   Qed.
 
-  Theorem indrep_bxp_switch : forall bxp bxp' xp ilist,
+  Theorem indrep_bxp_switch : forall bxp bxp' Fs xp ilist,
     BmapNBlocks bxp = BmapNBlocks bxp' ->
-    indrep bxp xp ilist <=p=> indrep bxp' xp ilist.
+    indrep bxp Fs xp ilist <=p=> indrep bxp' Fs xp ilist.
   Proof.
     intros. unfold indrep.
     repeat match goal with [|- context [indrep_n_tree ?i] ] =>
@@ -2255,9 +2678,9 @@ Module BlockPtr (BPtr : BlockPtrSig).
     reflexivity.
   Qed.
 
-  Theorem indrep_0 : forall bxp ir l,
+  Theorem indrep_0 : forall bxp Fs ir l,
     IRIndPtr ir = 0 -> IRDindPtr ir = 0 -> IRTindPtr ir = 0 ->
-    indrep bxp ir l <=p=> [[l = repeat $0 (NBlocks - NDirect)]].
+    indrep bxp Fs ir l <=p=> [[l = repeat $0 (NBlocks - NDirect)]] * [[ Fs <=p=> emp ]].
   Proof.
     unfold indrep. intros.
     repeat match goal with [H : _ = 0 |- _] => rewrite H end.
@@ -2274,13 +2697,13 @@ Module BlockPtr (BPtr : BlockPtrSig).
           repeat rewrite firstn_repeat by lia; f_equal; lia.
   Qed.
 
-  Lemma rep_keep_blocks : forall bxp ir ir' l,
+  Lemma rep_keep_blocks : forall bxp Fs ir ir' l,
     IRIndPtr ir = IRIndPtr ir' ->
     IRDindPtr ir = IRDindPtr ir' ->
     IRTindPtr ir = IRTindPtr ir' ->
     IRLen ir = IRLen ir' ->
     IRBlocks ir = IRBlocks ir' ->
-    rep bxp ir l =p=> rep bxp ir' l.
+    rep bxp Fs ir l =p=> rep bxp Fs ir' l.
   Proof.
     intros.
     unfold rep, indrep.
@@ -2290,8 +2713,8 @@ Module BlockPtr (BPtr : BlockPtrSig).
     reflexivity.
   Qed.
 
-  Theorem xform_indrep : forall xp ir l,
-    crash_xform (indrep xp ir l) <=p=> indrep xp ir l.
+  Theorem xform_indrep : forall xp Fs ir l,
+    crash_xform (indrep xp Fs ir l) <=p=> indrep xp Fs ir l.
   Proof.
     unfold indrep. intros.
     xform_norm.
@@ -2394,16 +2817,16 @@ Module BlockPtr (BPtr : BlockPtrSig).
     }.
 
   Theorem get_ok : forall lxp bxp ir off ms,
-    {< F Fm m0 m l,
+    {< F Fm IFs m0 sm m l,
     PRE:hm
-           LOG.rep lxp F (LOG.ActiveTxn m0 m) ms hm *
-           [[[ m ::: Fm * rep bxp ir l ]]] *
+           LOG.rep lxp F (LOG.ActiveTxn m0 m) ms sm hm *
+           [[[ m ::: Fm * rep bxp IFs ir l ]]] *
            [[ off < length l ]]
     POST:hm' RET:^(ms, r)
-           LOG.rep lxp F (LOG.ActiveTxn m0 m) ms hm' *
+           LOG.rep lxp F (LOG.ActiveTxn m0 m) ms sm hm' *
            [[ r = selN l off $0 ]]
     CRASH:hm'  exists ms',
-           LOG.rep lxp F (LOG.ActiveTxn m0 m) ms' hm'
+           LOG.rep lxp F (LOG.ActiveTxn m0 m) ms' sm hm'
     >} get lxp ir off ms.
   Proof.
     unfold get.
@@ -2427,15 +2850,15 @@ Module BlockPtr (BPtr : BlockPtrSig).
   Qed.
 
   Theorem read_ok : forall lxp bxp ir ms,
-    {< F Fm m0 m l,
+    {< F Fm IFs m0 sm m l,
     PRE:hm
-           LOG.rep lxp F (LOG.ActiveTxn m0 m) ms hm *
-           [[[ m ::: Fm * rep bxp ir l ]]]
+           LOG.rep lxp F (LOG.ActiveTxn m0 m) ms sm hm *
+           [[[ m ::: Fm * rep bxp IFs ir l ]]]
     POST:hm' RET:^(ms, r)
-           LOG.rep lxp F (LOG.ActiveTxn m0 m) ms hm' *
+           LOG.rep lxp F (LOG.ActiveTxn m0 m) ms sm hm' *
            [[ r = l ]]
     CRASH:hm'  exists ms',
-           LOG.rep lxp F (LOG.ActiveTxn m0 m) ms' hm'
+           LOG.rep lxp F (LOG.ActiveTxn m0 m) ms' sm hm'
     >} read lxp ir ms.
   Proof.
     unfold read.
@@ -2499,15 +2922,18 @@ Module BlockPtr (BPtr : BlockPtrSig).
 
   Theorem indshrink_helper_ok : forall lxp bxp bn nl indlvl ms,
     let start := fold_left plus (map (fun i => NIndirect ^ S i) (seq 0 indlvl)) 0 in
-    {< F Fm m0 m l freelist,
+    {< F Fm Fs IFs m0 sm m l freelist,
     PRE:hm
-           LOG.rep lxp F (LOG.ActiveTxn m0 m) (BALLOCC.MSLog ms) hm *
-           [[[ m ::: (Fm * indrep_n_tree indlvl bxp bn l * BALLOCC.rep bxp freelist ms) ]]]
-    POST:hm' RET:^(ms, r)  exists m' freelist' l',
-           LOG.rep lxp F (LOG.ActiveTxn m0 m') (BALLOCC.MSLog ms) hm' *
-           [[[ m' ::: (Fm * indrep_n_tree indlvl bxp r l' * BALLOCC.rep bxp freelist' ms) ]]] *
-           [[ l' = upd_range l (nl - start) (length l - (nl - start)) $0 ]] * [[ incl freelist freelist' ]]
-    CRASH:hm'  LOG.intact lxp F m0 hm'
+           LOG.rep lxp F (LOG.ActiveTxn m0 m) (BALLOCC.MSLog ms) sm hm *
+           [[[ m ::: (Fm * indrep_n_tree indlvl IFs bxp bn l * BALLOCC.rep bxp freelist ms) ]]] *
+           [[ (Fs * IFs * BALLOCC.smrep freelist)%pred sm ]]
+    POST:hm' RET:^(ms, r)  exists m' freelist' IFs' l',
+           LOG.rep lxp F (LOG.ActiveTxn m0 m') (BALLOCC.MSLog ms) sm hm' *
+           [[[ m' ::: (Fm * indrep_n_tree indlvl IFs bxp r l' * BALLOCC.rep bxp freelist' ms) ]]] *
+           [[ l' = upd_range l (nl - start) (length l - (nl - start)) $0 ]] *
+           [[ (Fs * IFs' * BALLOCC.smrep freelist')%pred sm ]] *
+           [[ incl freelist freelist' ]]
+    CRASH:hm'  LOG.intact lxp F m0 sm hm'
     >} indshrink_helper indlvl lxp bxp bn nl ms.
   Proof.
     unfold indshrink_helper.
@@ -2520,19 +2946,23 @@ Module BlockPtr (BPtr : BlockPtrSig).
   Local Hint Extern 1 ({{_}} Bind (indshrink_helper _ _ _ _ _ _ ) _) => apply indshrink_helper_ok : prog.
 
   Theorem indshrink_ok : forall lxp bxp ir nl ms,
-    {< F Fm m0 m l0 l1 l2 freelist,
+    {< F Fm Fs m0 sm m l0 l1 l2 freelist,
     PRE:hm
-           LOG.rep lxp F (LOG.ActiveTxn m0 m) (BALLOCC.MSLog ms) hm * [[ nl <= length (l0 ++ l1 ++ l2) ]] *
-           [[[ m ::: (Fm * indrep_n_tree 0 bxp (IRIndPtr ir) l0 *
-                           indrep_n_tree 1 bxp (IRDindPtr ir) l1 *
-                           indrep_n_tree 2 bxp (IRTindPtr ir) l2 * BALLOCC.rep bxp freelist ms) ]]]
+           LOG.rep lxp F (LOG.ActiveTxn m0 m) (BALLOCC.MSLog ms) sm hm *
+           [[ nl <= length (l0 ++ l1 ++ l2) ]] *
+           [[[ m ::: (Fm * indrep_n_tree 0 bxp IFs0 (IRIndPtr ir) l0 *
+                           indrep_n_tree 1 bxp IFs1 (IRDindPtr ir) l1 *
+                           indrep_n_tree 2 bxp IFs2 (IRTindPtr ir) l2 *
+                           BALLOCC.rep bxp freelist ms) ]]] *
+           [[ (Fs * IFs0 * IFs1 * IFs2 * BALLOCC.smrep freelist)%sm ]]
     POST:hm' RET:^(ms, indptr', dindptr', tindptr')
-           exists m' freelist' l0' l1' l2',
-           LOG.rep lxp F (LOG.ActiveTxn m0 m') (BALLOCC.MSLog ms) hm' *
-           [[[ m' ::: (Fm * indrep_n_tree 0 bxp indptr' l0' *
-                            indrep_n_tree 1 bxp dindptr' l1' *
-                            indrep_n_tree 2 bxp tindptr' l2' * BALLOCC.rep bxp freelist' ms) ]]] *
+           exists m' freelist' l0' l1' l2' IFs0' IFs1' IFs2',
+           LOG.rep lxp F (LOG.ActiveTxn m0 m') (BALLOCC.MSLog ms) sm hm' *
+           [[[ m' ::: (Fm * indrep_n_tree 0 bxp IFs0' indptr' l0' *
+                            indrep_n_tree 1 bxp IFs1' dindptr' l1' *
+                            indrep_n_tree 2 bxp IFs2' tindptr' l2' * BALLOCC.rep bxp freelist' ms) ]]] *
            [[ l0' ++ l1' ++ l2' = upd_range (l0 ++ l1 ++ l2) nl (length (l0 ++ l1 ++ l2) - nl) $0 ]] *
+           [[ (Fs * IFs0' * IFs1' * IFs2 * BALLOCC.smrep freelist)%sm ]] *
            [[ incl freelist freelist' ]]
     CRASH:hm'  LOG.intact lxp F m0 hm'
     >} indshrink lxp bxp ir nl ms.
